---
title: 单变量微积分：泰勒公式
date: 2019-02-02 10:04:57
tags:
  - Calculus
---

### Taylor's Formula
$$f(x) = \sum_{n = 0}^{\infty} \frac{f^{n}(0)}{n!} x^{n} \quad |x| \lt R$$

<!--more-->

$f(x) = a_{0} + a_{1} x + a_{2} x^{2} + a_{3} x^{3} + ...$
$f'(x) = a_{1} + 2a_{2} x + 3a_{3} x^{2} + ...$
$f''(x) = 2a_{2} + 3 \cdot 2a_{3} x + ...$
$f'''(x) = 3 \cdot 2a_{3} + ...$
$f'''(0) = 3 \cdot 2 a_{3} \to \frac{f'''(0)}{3 \cdot 2 \cdot 1} = a_{3}$
> In general
> $$a_{n} = \frac{f^{n}(0)}{n!}$$

- $f(x) = e^{x}$
  $f'(x) = e^{x} \quad f''(x) = e^{x} \quad f^{n}(x) = e^{x}$
  $e^{x} \mid_{x = 0} = 1$
  $e^{x} = \sum_{n = 0}^{\infty} \frac{1}{n!} x^{n} \quad R = \infty$
  $e = e^{1} = 1 + 1 + \frac{1}{2!} + \frac{1}{3!} + ...$

- $\sin x = x - \frac{x^{3}}{3!} + \frac{x^{5}}{5!} - \frac{x^{7}}{7!} + ... \quad R = \infty$
- $\cos x = 1 - \frac{x^{2}}{2!} + \frac{x^{4}}{4!} - \frac{x^{6}}{6!} + ... \quad R = \infty$
- $\frac{1}{1 - x} = 1 + x + x^{2} + x^{3} + ... \quad R = 1$
- $\frac{1}{1 + x} = 1 - x + x^{2} - x^{3} + ... \quad R = 1$

### Rules
- Multiply
  $x \sin x = x^{2} - \frac{x^{4}}{3!} + \frac{x^{6}}{5!} - \frac{x^{8}}{7!} + ... \quad R = \infty$
- Differentiate
  $\cos x = \sin'x = 1 - \frac{3x^{2}}{3!} + \frac{5x^{4}}{5!} - ... = 1 - \frac{x^{2}}{2!} + \frac{x^{4}}{4!} - ... \quad R = \infty$
- Integrate
  $\ln (1 + x) = \int_{0}^{x} \frac{dt}{1 + t}  = \int_{0}^{x} (1 - t + t^{2} - t^{3} + ...) dt$
  $= (t - \frac{t^{2}}{2} + \frac{t^{3}}{3} - \frac{t^{4}}{4} + ...)_{0}^{x} = x - \frac{x^{2}}{2} + \frac{x^{3}}{3} - \frac{x^{4}}{4} + ... \quad R = 1$
- Subsitute
  $e^{-t^{2}} = 1 + (-t^{2}) + \frac{(-t^{2})^{2}}{2!} + \frac{(-t^{2})^{3}}{3!} + ... = 1 - t^{2} + \frac{t^{4}}{2!} - \frac{t^{6}}{3!} + ... \quad x = -t^{2}\ in\ e^{x} $