---
title: '单变量微积分：微分与不定积分'
date: 2018-12-29 18:37:28
tags:
  - Calculus
---

### 微分(Differential)
$y = f(x)$
$Differential\ of\ y\ (f):\ dy = f'(x)dx$
> Leibniz's interpretation of derivative as a ratio of infinitesimal(无穷小量)
> $dy = f'(x)dx \Leftrightarrow \frac{dy}{dx} = f'(x)$

<!--more-->

- Use in linear approximation
> $dx\ replace\ \Delta x \quad when \quad \Delta x \to 0$
> $dy\ replace\ \Delta y$

  - Example $(64.1)^{\frac{1}{3}} \approx ?$
    $y = x^{\frac{1}{3}},\ dy = \frac{1}{3}x^{-\frac{2}{3}}dx$
    $At\ x = 64,\ y = 64^{\frac{1}{3}} = 4$
    $dy = \frac{1}{3}64^{-\frac{2}{3}} = \frac{1}{3} \frac{1}{16}dx = \frac{1}{48}dx$
    $x = 64,\ x+dx=64.1 \to dx=0.1$
    $(64.1)^{\frac{1}{3}} = y + \Delta y \approx y + dy = 4 + \frac{1}{48}dx \approx 4.002$
  
  - Compare to previous notation
    $f(x) \approx f(x_{0}) + f'(x_{0})(x-x_{0})$
    $x_{0} = 64,\ f(x)=x^{\frac{1}{3}}$
    $f(x_{0}) = f(64) = 4$
    $f'(x_{0})=\frac{1}{3}x_{0}^{-\frac{2}{3}} = \frac{1}{48}$
    $x^{\frac{1}{3}} \approx 4 + \frac{1}{48}(x-64) \quad when \quad x\ near\ x_{0}$
    $(64.1)^{\frac{1}{3}} \approx 4 + \frac{1}{48} \frac{1}{10} \approx 4.002$

### 不定积分(Indefinite Integral)
#### Antiderivative
$$G(x) = \int g(x) dx$$
> $G(x)\ antiderivative\ of\ g = indefinite\ integral\ of\ g$
> $\int\ is\ integral\ sign$

#### 常用公式
- $\int \sin x dx = -\cos x + c$
- $\int x^{a} dx = \frac{1}{a+1} x^{a+1} + c (a \neq -1)$
- $\int \frac{1}{x} dx = \ln \left| x \right| + c$
- $\int \sec^{2} x dx = \tan x + c$
- $\int \frac{dx}{\sqrt{1-x^{2}}} = \sin^{-1} x + c$
- $\int \frac{dx}{1+x^2} = \tan^{-1} x + c$

> $If\ F' = G',\ then\ F(x) = G(x) + c$
> PROOF
> $If\ F' = G',\ then\ (F-G)' = F'-G'=0,\ hence\ F(x)-G(x)=c$

#### 换元法(Method of Subsititution)
##### 第一类换元
$$\int f[\varphi (x)] \varphi'(x) dx = [\int f(u) du]_{u=\varphi (x)}$$

- Example 1 $\int x^{3}(x^{4}+2)^{5} dx$
$u = x^{4} + 2 \quad du = 4x^{3} dx$
$\int x^{3}(x^{4}+2)^{5} dx = \int u^{5} \frac{1}{4} du = \frac{1}{24}u^{6}+c = \frac{1}{24} (x^{4}+2)^{6} + c$
- Example 2 $\int \frac{x}{\sqrt{1+x^{2}}} dx = \sqrt{1+x^{2}} + c$
$u = 1 + x^{2} \quad du = 2x dx$
$\int u^{-\frac{1}{2}} du$
- Example3 $\int \sin x \cos x dx = \frac{1}{2} sin^{2}x + c$
- Example4 $\int \frac{dx}{x \ln x} = \int \frac{1}{\ln x} d \ln x = \ln\left|\ln x \right| + c$

##### 第二类换元
$$\int f(x) dx = [\int f[\psi (t)] \psi'(t) dt]_{t=\psi^{-1}(x)}$$
> $x = \psi(t)$ 单调可导

### 微分方程(Differential Equation)
#### 分离变量法
> $\frac{dy}{dx} = f(x)g(y)$
> $\frac{dy}{g(y)} = f(x)dx$
> $H(y) = \int \frac{dy}{g(y)} \quad F(x) = \int f(x) dx$
> $H(y) = F(x) + c$

- Example1 $\frac{dy}{dx} = f(x)$
$y = \int f(x) dx$

- Example2 $(\frac{d}{dx}+x)y = 0$
$\frac{dy}{dx} = -xy$
$\frac{dy}{y} = -x dx$
$\int \frac{dy}{y} = \int -x dx$
$\ln y = -\frac{x^{2}}{2}+c\ (y \gt 0)$
$y = e^{-\frac{x^{2}}{2}+c} \to y = Ae^{-\frac{x^{2}}{2}}$
$\ln\left|y\right| = -\frac{x^{2}}{2} + c \quad y \neq 0$
$\left|y\right| = Ae^{-\frac{x^{2}}{2}} \quad A \gt 0$
$y = \pm Ae^{-\frac{x^{2}}{2}} \quad a = \pm A$
$when\ y = 0,\ a = 0$
$y = ae^{-\frac{x^{2}}{2}},\ a \gt 0\ a \lt 0\ a = 0$ 通解
